update some agda and Coq

Coq/Coq24.v
@@ -12,5 +12,126 @@ From Coq Require Import omega.Omega.
 Add LoadPath "C:\Users\ycy12\Documents\Workspace\LEARNING-STUFF\Coq".
 Load Coq19.
 
+Definition Assertion := state -> Prop.
+Definition assert_implies (P Q : Assertion) : Prop :=
+  ∀st, P st → Q st.
+Notation "P ->> Q" := (assert_implies P Q)
+                      (at level 80) : hoare_spec_scope.
+Open Scope hoare_spec_scope.
 
+Notation "P <<->> Q" :=
+  (P ->> Q ∧ Q ->> P) (at level 80) : hoare_spec_scope.
+
+Definition hoare_triple
+           (P : Assertion) (c : com) (Q : Assertion) : Prop :=
+  ∀st st',
+     st =[ c ]⇒ st' →
+     P st →
+     Q st'.
+
+Notation "{{ P }} c {{ Q }}" :=
+  (hoare_triple P c Q) (at level 90, c at next level)
+  : hoare_spec_scope.
+
+Theorem hoare_post_true : ∀(P Q : Assertion) c,
+  (∀st, Q st) →
+  {{P}} c {{Q}}.
+Proof.
+  intros P Q c H. unfold hoare_triple.
+  intros st st' Heval HP.
+  apply H. Qed.
+
+Theorem hoare_pre_false : ∀(P Q : Assertion) c,
+  (∀st, ¬(P st)) →
+  {{P}} c {{Q}}.
+Proof.
+  intros P Q c H. unfold hoare_triple.
+  intros st st' Heval HP.
+  unfold not in H. apply H in HP.
+  inversion HP. Qed.
+
+Definition assn_sub X a P : Assertion :=
+  fun (st : state) =>
+    P (X !-> aeval st a ; st).
+Notation "P [ X ⊢> a ]" := (assn_sub X a P)
+                             (at level 10, X at next level).
+
+Theorem hoare_asgn : ∀Q X a,
+  {{Q [X ⊢> a]}} X ::= a {{Q}}.
+Proof.
+  intros Q X a.
+  unfold assn_sub. unfold hoare_triple.
+  intros. inversion H;subst. apply H0.
+Qed.
+
+Lemma assn_sub_ex1 : {{(fun st => st X <= 10) [X ⊢> 2 * X] }}
+                       X ::= 2 * X
+                     {{fun st => st X <= 10}}.
+Proof.
+  apply hoare_asgn.
+Qed.
+
+Lemma assn_sub_ex2 : {{(fun st => st X >= 0 /\ st X <= 5) [X ⊢> 3]}}
+                       X ::= 3
+                     {{fun st => st X >= 0 /\ st X <= 5}}.
+Proof.
+  apply hoare_asgn.
+Qed.
+Axiom functional_extensionality : ∀ {X Y: Type} {f g : X → Y}, (∀ (x:X), f x = g x) → f = g.
+
+Lemma beq_stringP : ∀ x y, reflect (x = y) (beq_string x y).
+Proof.
+  intros. destruct (beq_string x y) eqn:HS.
+  - apply ReflectT. apply beq_string_true_iff. auto.
+  - apply ReflectF. apply beq_string_false_iff. auto.
+Qed.
+
+Theorem t_update_same : ∀(A : Type) (m : total_map A) x,
+    (x !-> m x ; m) = m.
+Proof.
+  intros. apply functional_extensionality.
+  intros. unfold t_update.
+  destruct (beq_stringP x x0).
+  - rewrite e. auto.
+  - auto.
+Qed.
+
+Lemma t_update_shadow : ∀(A : Type) (m : total_map A) x v1 v2,
+    (x !-> v2 ; x !-> v1 ; m) = (x !-> v2 ; m).
+Proof.
+  intros.
+  apply functional_extensionality.
+  intros. unfold t_update.
+  destruct (beq_string x x0) eqn:HE.
+  - auto.
+  - auto.
+Qed.
+
+Theorem hoare_asgn_fwd :
+  ∀m a P,
+  {{fun st => P st ∧ st X = m}}
+    X ::= a
+  {{fun st => P (X !-> m ; st)
+           ∧ st X = aeval (X !-> m ; st) a }}.
+Proof.
+  intros. unfold hoare_triple. intros.
+  inversion H. subst. destruct H0.
+  subst. rewrite t_update_shadow. rewrite t_update_same. split.
+  - auto.
+  - rewrite t_update_eq. auto.
+Qed.
+
+Theorem hoare_asgn_fwd_exists :
+  ∀a P,
+  {{fun st => P st}}
+    X ::= a
+  {{fun st => ∃m, P (X !-> m ; st) ∧
+                st X = aeval (X !-> m ; st) a }}.
+Proof.
+  intros a P.
+  unfold hoare_triple. intros.
+  inversion H;subst. exists (st X).
+  rewrite t_update_shadow. rewrite t_update_same. split.
+  auto. rewrite t_update_eq. auto.
+Qed.
 
