Agda/Ag05.agda
@@ -2,6 +2,7 @@ module Ag05 where
 
 open import Agda.Builtin.Nat
 open import Agda.Builtin.Equality
+open import Agda.Builtin.Bool
 
 {-
 data _≡_ {A : Set} (x : A) : A → Set where
@@ -10,11 +11,75 @@ data _≡_ {A : Set} (x : A) : A → Set where
 data Refine : (A : Set) → (A → Set) → Set where
   MkRefine : ∀ {A : Set} {f : A → Set} → (a : A) → (f a) → Refine A f
 
+data _∧_ : Set → Set → Set where
+  and : ∀ (A B : Set) → A ∧ B 
+
+-- hl-suc : ∀ {a : Nat} → Refine Nat (λ )
+
 silly : Set
 silly = Refine Nat (_≡_ 0)
 
 sillySon : silly
 sillySon = MkRefine zero refl
 
+data _≤_ : Nat → Nat → Set where
+  z≤s : ∀ {b   : Nat} → 0 ≤ b
+  s≤s : ∀ {m n : Nat} → m ≤ n → suc m ≤ suc n
 
+data le-Total (x y : Nat) : Set where
+  le-left  : x ≤ y → le-Total x y
+  le-right : y ≤ x → le-Total x y
+
+le : Nat → Nat → Bool
+le zero    zero    = true
+le zero    (suc n) = true
+le (suc m) zero    = false
+le (suc m) (suc n) = le m n
+
+le-wtf : ∀ (x y : Nat) → le-Total x y
+le-wtf zero    zero    = le-left z≤s
+le-wtf zero    (suc y) = le-left z≤s
+le-wtf (suc x) zero    = le-right z≤s
+le-wtf (suc x) (suc y) with le-wtf x y
+...                    | le-left  P = le-left  (s≤s P)
+...                    | le-right Q = le-right (s≤s Q)
+{- with le x y -- x ≤ y
+...        | true  = {!!}
+...        | false = {!!}
+-}
+_⟨_⟩ : (A : Set) → (A → Set) → Set
+_⟨_⟩ = Refine
+
+and-refine : ∀ {A : Set} (f g : A → Set)
+           → (a : A) → f a → g a
+           → Refine A (λ x → (f x) ∧ (g x))
+and-refine f g x Pa Pb = MkRefine x (and (f x) (g x))
+
+hSuc : ∀ {m : Nat} → ( Nat ⟨ (λ x → x ≤ m     ) ⟩ )
+                   → ( Nat ⟨ (λ x → x ≤ suc m ) ⟩ )
+hSuc (MkRefine a P) = MkRefine (suc a) (s≤s P)
+
+postulate
+  ≤-trans : ∀ {x y z : Nat} → x ≤ y → y ≤ z → x ≤ z
+
+min : ∀ {m n : Nat} → ( Nat ⟨ (λ x → x ≤ m)             ⟩ )
+                    → ( Nat ⟨ (λ x → x ≤ n)             ⟩ )
+                    → ( Nat ⟨ (λ x → (x ≤ m) ∧ (x ≤ n)) ⟩ )
+min (MkRefine a Pa) (MkRefine b Pb) with le-wtf a b
+...                    {- a ≤ b -}  | le-left  P = {!and-refine ? ? Pa ? !}
+...                    {- b ≤ a -}  | le-right Q = {!and-refine _ _ ? Pb !}
+{- 
+with le-Total a b
+...                                 | le-left  a = {!!}
+...                                 | le-right b = ? -}
+{-
+min {m} {n} (MkRefine a P₀) (MkRefine b P₁) with (le a b)
+...                                 | true  = {!!}
+...                                 | false = {!!}
+-}
+{-
+min {m} {n} (MkRefine zero x)    (MkRefine b y)    = MkRefine 0 (and (zero ≤ m) (zero ≤ n))
+min {m} {n} (MkRefine (suc a) x) (MkRefine zero y) = MkRefine 0 (and (zero ≤ m) (zero ≤ n))
+min {suc m} {suc n} (MkRefine (suc a) x) (MkRefine (suc b) y) = {!hSuc (min (MkRefine a ?) (MkRefine b ?))!}
+-}
 
