Agda/Ag06.agda
@@ -1,0 +1,9 @@
+module Ag06 where
+
+import Relation.Binary.PropositionalEquality as Eq
+open Eq using (_≡_; refl; cong; cong-app)
+open Eq.≡-Reasoning
+open import Data.Nat using (ℕ; zero; suc; _+_)
+open import Data.Nat.Properties using (+-comm)
+
+
