Agda/Ag07.agda
@@ -1,0 +1,35 @@
+module Ag07 where
+
+open import IO
+
+data W (A : Set) (B : A → Set) : Set where
+  sup : (a : A) → (b : B a → W A B) → W A B
+
+module WBinTree where
+  data Tree : Set where
+    Leaf : Tree
+    Node : Tree
+  
+  data Direction : Set where
+    Left  : Direction
+    Right : Direction
+
+  data Bottom : Set where
+
+  void : ∀ {A : Set} → Bottom → A
+  void ()
+
+  binTree : Tree → Set
+  binTree Leaf = Bottom
+  binTree Node = Direction
+
+  BinTree : Set
+  BinTree = W Tree binTree
+
+  leaf : BinTree
+  leaf = sup Leaf void
+
+  node : BinTree → BinTree → BinTree
+  node x y = sup Node λ {
+    Left  → x ;
+    Right → y }
